---
title: "Assignment 2 Question 2"
output: pdf_document
author: Sheen Thusoo
---

```{r setup, include=FALSE}
knitr::opts_chunk$set(echo = TRUE)
```

# Part a)

$$
L(\boldsymbol\theta;y_1,...,y_n) = f_{\boldsymbol\theta}(y_1)\times...\times f_{\boldsymbol\theta}(y_n)
$$

$$
\ell(\boldsymbol\theta;y_1,...,y_n) = \log\big(L(\boldsymbol\theta;y_1,...,y_n)\big)
$$
$$
\ell(\boldsymbol\theta;y_1,...,y_n) = \log(f_{\boldsymbol\theta}(y_1)\times...\times f_{\boldsymbol\theta}(y_n))
$$


$$
\ell(\boldsymbol\theta;y_1,...,y_n) = \log(f_{\boldsymbol\theta}(y_1)) + ... + log(f_{\boldsymbol\theta}(y_n))
$$


$$
\ell(\boldsymbol\theta;y_1,...,y_n) = \sum_{i \in P} \log(f_{\boldsymbol\theta}(y_i))
$$

$$
f(y) = \frac{\beta^\alpha y^{\alpha-1}}{\Gamma(\alpha)}\exp(-y\beta)
$$


$$
\ell(\boldsymbol\theta;y_1,...,y_n) = \sum_{i \in P} \log \left( \frac{\beta^\alpha y_i^{\alpha-1}}{\Gamma(\alpha)}\exp(-y_i\beta) \right)
$$

Therefore the log-likelihood function of the parameter vector $\theta = (\alpha, \beta)$ is,

$$
\ell(\boldsymbol\theta;y_1,...,y_n) = \sum_{i \in P} \alpha \log(\beta) + (\alpha-1) \log(y_i) - \log(\Gamma(\alpha)) - y_i\beta
$$

